pulse/lib/steel/pulse/Pulse.Prover.Substs.fst
@@ -202,6 +202,33 @@ let rec ss_comp_commutes (c:comp) (ss:ss_t)
   | [] -> ()
   | y::tl -> ss_comp_commutes (subst_comp c [ NT y (Map.sel ss.m y) ]) (tail ss)
 
+let rec nt_substs_st_comp_commutes (s:st_comp) (nts:nt_substs)
+  : Lemma (ensures
+             nt_subst_st_comp s nts ==
+             { s with res = nt_subst_term s.res nts;
+                      pre = nt_subst_term s.pre nts;
+                      post = nt_subst_term s.post nts; })  // no shifting required
+          (decreases nts)
+          [SMTPat (nt_subst_st_comp s nts)] =
+  match nts with
+  | [] -> ()
+  | (NT x e)::nts_tl -> nt_substs_st_comp_commutes (nt_subst_st_comp s [ NT x e ]) nts_tl
+
+let rec nt_subst_comp_commutes (c:comp) (nts:nt_substs)
+  : Lemma (ensures
+             (let r = nt_subst_comp c nts in
+              (C_Tot? c ==> r == C_Tot (nt_subst_term (comp_res c) nts)) /\
+              (C_ST? c ==> r == C_ST (nt_subst_st_comp (st_comp_of_comp c) nts)) /\
+              (C_STAtomic? c ==> r == C_STAtomic (nt_subst_term (comp_inames c) nts)
+                                                 (nt_subst_st_comp (st_comp_of_comp c) nts)) /\
+              (C_STGhost? c ==> r == C_STGhost (nt_subst_term (comp_inames c) nts)
+                                               (nt_subst_st_comp (st_comp_of_comp c) nts))))
+          (decreases nts)
+          [SMTPat (nt_subst_comp c nts)] =
+  match nts with
+  | [] -> ()
+  | (NT x e)::nts_tl -> nt_subst_comp_commutes (nt_subst_comp c [ NT x e ]) nts_tl
+
 let rec is_permutation (nts:nt_substs) (ss:ss_t) : Type0 =
   match nts, ss.l with
   | [], [] -> True
@@ -277,191 +304,18 @@ let rec st_typing_nt_substs
       (subst_env uvs_rest [ NT x e ])
       (subst_env g' [ NT x e ])
       t_typing nts_rest
-   
 
-// let well_typed_nt_substs 
+let st_typing_nt_substs_derived
+  (g:env) (uvs:env { disjoint uvs g })
+  (#t:st_term) (#c:comp_st) (t_typing:st_typing (push_env g uvs) t c)
+  (ss:nt_substs { well_typed_nt_substs g uvs ss })
+  : st_typing g (nt_subst_st_term t ss) (nt_subst_comp c ss) =
 
-// let permutation #uvs (ss1 ss2:ss_t uvs) =
-//   Map.equal ss1.m ss2.m
-
-// let rec ss_term_permutation #uvs (t:term) (ss1 ss2:ss_t uvs)
-//   : Lemma (requires permutation ss1 ss2)
-//           (ensures ) 
-
-// let rec nt_subst_st_comp_commutes (s:st_comp) (ss:nt_substs)
-//   : Lemma (ensures nt_subst_st_comp s ss ==
-//            { s with res = nt_subst_term s.res ss;
-//                     pre = nt_subst_term s.pre ss;
-//                     post = nt_subst_term s.post ss; })
-//           (decreases L.length ss) =
-//   match ss with
-//   | [] -> ()
-//   | (NT x e)::tl ->
-//     nt_subst_st_comp_commutes (subst_st_comp s [ NT x e ]) tl
-
-
-// let rec nt_subst_comp_commutes (c:comp) (ss:nt_substs)
-//   : Lemma (ensures (let r = nt_subst_comp c ss in
-//            (C_Tot? c ==> r == C_Tot (nt_subst_term (comp_res c) ss)) /\
-//            (C_ST? c ==> r == C_ST (nt_subst_st_comp (st_comp_of_comp c) ss)) /\
-//            (C_STAtomic? c ==> r == C_STAtomic (nt_subst_term (comp_inames c) ss)
-//                                               (nt_subst_st_comp (st_comp_of_comp c) ss)) /\
-//            (C_STGhost? c ==> r == C_STGhost (nt_subst_term (comp_inames c) ss)
-//                                             (nt_subst_st_comp (st_comp_of_comp c) ss))))
-//           (decreases L.length ss) =
-  
-//   match ss with
-//   | [] -> ()
-//   | (NT x e)::tl ->
-//     nt_subst_comp_commutes (subst_comp c [ NT x e ]) tl
-
-// let rec nt_subst_term_compose (t:term) (ss1 ss2:nt_substs)
-// : Lemma (ensures nt_subst_term (nt_subst_term t ss1) ss2 ==
-//                  nt_subst_term t (compose_nt_substs ss1 ss2))
-//         (decreases L.length ss1) =
-
-// match ss1 with
-// | [] -> ()
-// | (NT x e)::tl -> nt_subst_term_compose (subst_term t [ NT x e ]) tl ss2
-
-// let rec nt_subst_st_term_compose (t:st_term) (ss1 ss2:nt_substs)
-// : Lemma (ensures nt_subst_st_term (nt_subst_st_term t ss1) ss2 ==
-//                  nt_subst_st_term t (compose_nt_substs ss1 ss2))
-//         (decreases L.length ss1) =
-
-// match ss1 with
-// | [] -> ()
-// | (NT x e)::tl -> nt_subst_st_term_compose (subst_st_term t [ NT x e ]) tl ss2
-
-// let rec nt_subst_comp_compose (c:comp) (ss1 ss2:nt_substs)
-// : Lemma (ensures nt_subst_comp (nt_subst_comp c ss1) ss2 ==
-//                  nt_subst_comp c (compose_nt_substs ss1 ss2))
-//         (decreases L.length ss1) =
-
-// match ss1 with
-// | [] -> ()
-// | (NT x e)::tl -> nt_subst_comp_compose (subst_comp c [ NT x e ]) tl ss2
-
-// let coerce_eq (#a #b:Type) (x:a) (_:squash (a === b)) : y:b{y == x} = x
-
-// let rec st_typing_nt_substs
-//   (g:env) (uvs:env) (g':env { pairwise_disjoint g uvs g' })
-//   (#t:st_term) (#c:comp_st) (t_typing:st_typing (push_env g (push_env uvs g')) t c)
-//   (ss:nt_substs { well_typed_ss g uvs ss })
-// : Tot (st_typing (push_env g (nt_subst_env g' ss)) (nt_subst_st_term t ss) (nt_subst_comp c ss))
-//       (decreases L.length ss) =
-
-// match bindings uvs with
-// | [] ->
-//   assert (equal (push_env uvs g') g');
-//   t_typing
-
-// | _ ->
-//   let x, ty, uvs' = remove_binding uvs in
-//   let (NT y e)::ss' = ss in
-//   let e_typing = FStar.IndefiniteDescription.elim_squash #(tot_typing g e ty) () in
-//   push_env_assoc (singleton_env (fstar_env uvs) x ty) uvs' g';
-//   let t_typing
-//     : st_typing (push_env g (push_env (singleton_env (fstar_env g) x ty) (push_env uvs' g'))) t c
-//     = coerce_eq t_typing () in
-//   let t_typing
-//     : st_typing (push_env g (subst_env (push_env uvs' g') [ NT y e ]))
-//                 (subst_st_term t [ NT y e ])
-//                 (subst_comp c [ NT y e ])
-//     = st_typing_subst g x ty (push_env uvs' g') e_typing t_typing in
-
-//   assume (subst_env (push_env uvs' g') [ NT y e ] ==
-//           push_env (subst_env uvs' [ NT y e ]) (subst_env g' [ NT y e ]));
-
-//   st_typing_nt_substs g
-//     (subst_env uvs' [ NT y e ])
-//     (subst_env g' [ NT y e ])
-//     t_typing ss'
-
-// let vprop_equiv_nt_substs
-//   (g:env) (uvs:env) (g':env { pairwise_disjoint g uvs g' })
-//   (#p1 #p2:vprop) (veq:vprop_equiv (push_env g (push_env uvs g')) p1 p2)
-//   (ss:nt_substs { well_typed_ss g uvs ss })
-// : vprop_equiv (push_env g (nt_subst_env g' ss)) (nt_subst_term p1 ss) (nt_subst_term p2 ss) =
-
-// admit ()
+  let g' = mk_env (fstar_env g) in
+  assert (equal (push_env g (push_env uvs g')) (push_env g uvs));
+  let d = st_typing_nt_substs g uvs g' (coerce_eq t_typing ()) ss in
+  assume (nt_subst_env g' ss == g');
+  assert (equal (push_env g (nt_subst_env g' ss)) g);
+  d
 
 let vprop_equiv_nt_substs_derived _ _ _ _ = admit ()
-
-
-// type map = m:Map.t var term {
-//   forall (x:var). (~ (Map.contains m x)) ==> Map.sel m x == tm_unknown
-// }
-
-// let related (l:list (var & term)) (m:map) =
-//   (forall (b:var & term).
-//           L.memP b l ==> (Map.contains m (fst b) /\
-//                           Map.sel m (fst b) == snd b)) /\
-  
-//   (forall (x:var). Map.contains m x ==> L.memP (x, Map.sel m x) l)
-
-// noeq
-// type t = {
-//   l : list (var & term);
-//   m : m:map { related l m }
-// }
-
-// let rec as_nt_substs_aux (l:list (var & term)) : nt_substs =
-//   match l with
-//   | [] -> []
-//   | (x, t)::tl -> (NT x t)::(as_nt_substs_aux tl)
-
-// let as_nt_substs s = as_nt_substs_aux s.l
-
-// let as_map s = s.m
-
-// let empty = {
-//   l = [];
-//   m = Map.const_on Set.empty tm_unknown;
-// }
-
-// let empty_dom () = assert (Set.equal (dom empty) Set.empty)
-
-// let singleton (x:var) (t:term) = {
-//   l = [ (x, t) ];
-//   m = Map.upd (Map.const_on Set.empty tm_unknown) x t;
-// }
-
-// //
-// // TODO: Move to ulib
-// //
-// let rec append_memP (#a:Type) (l1 l2:list a) (x:a)
-//   : Lemma (L.memP x (l1 @ l2) <==> (L.memP x l1 \/ L.memP x l2))
-//           [SMTPat (L.memP x (l1 @ l2))] =
-//   match l1 with
-//   | [] -> ()
-//   | _::tl -> append_memP tl l2 x
-
-// let push s1 s2 = {
-//   l = s1.l @ s2.l;
-//   m = Map.concat s1.m s2.m;
-// }
-
-// let push_as_map _ _ = ()
-
-// let check_well_typedness g uvs ss = admit (); true
-
-// // let t _ = magic ()
-// // let as_subst _ = magic ()
-// // let as_map _ = magic ()
-// // let subst_as_map _ = admit ()
-// // let equal_elim _ _ = admit ()
-// // let empty _ = magic ()
-// // let empty_dom _ = admit ()
-// // let singleton _ = magic ()
-// // let singleton_dom _ _ = admit ()
-// // let push _ _ = magic ()
-// // let push_substs_as_map _ _ = admit ()
-// // let push_subst_term _ _ _ = admit ()
-// // let push_subst_st_term _ _ _ = admit ()
-// // let push_subst_comp _ _ _ = admit ()
-// // let subst_closed_term _ _ = admit ()
-// // let subst_closed_st_term _ _ = admit ()
-// // let subst_closed_comp _ _ = admit ()
-// // let diff _ _ = magic ()
-// // let diff_push _ _ = admit ()
