pulse/lib/steel/pulse/Pulse.Prover.fsti
@@ -15,6 +15,6 @@ val prove
 
   : T.Tac (g1 : env { g1 `env_extends` g } &
            uvs1 : env { uvs1 `env_extends` uvs /\ disjoint uvs1 g1 } &
-           ss1 : PS.ss_t { well_typed_ss ss1 uvs1 g1 } &
+           nts1 : PS.nt_substs { PS.well_typed_nt_substs g1 uvs1 nts1 } &
            remaining_ctxt : vprop &
-           continuation_elaborator g ctxt g1 (ss1.(goals) * remaining_ctxt))
+           continuation_elaborator g ctxt g1 ((PS.nt_subst_term goals nts1) * remaining_ctxt))
